extract mainfunction and costfunction from MainFunc constructor, update Zulib

src/Blockchain.Tests/ValidateBlockTests.fs
@@ -607,7 +607,7 @@ let ``block with a contract activation is added to chain``() =
 
     let contract = {
         hash = cHash
-        fn = fun _ _ _ _  tx -> Ok (tx,None)
+        mainFn = fun tx _ _ _ _  -> Ok (tx,None)
         costFn = fun _ _ _ _ -> 1L
         expiry=1002ul
         size=String.length sampleContractCode |> uint32
