src/Consensus.Tests/BlockTests.fs
@@ -253,7 +253,7 @@ let ``can connect block with a contract``() =
     let contract : Contract.T =
         {
             hash=Contract.computeHash SampleContract.sampleContractCode
-            fn= fun _ _ _ _ tx -> Ok (tx,None)
+            mainFn = fun tx _ _ _ _ -> Ok (tx,None)
             costFn = fun _ _ _ _ -> 0L
             expiry=1001ul
             size=String.length SampleContract.sampleContractCode |> uint32
@@ -286,7 +286,7 @@ let ``block with invalid contract failed connecting``() =
     let contract : Contract.T =
         {
             hash=Contract.computeHash "ada"
-            fn= fun _ _ _ _ tx -> Ok (tx,None)
+            mainFn = fun tx _ _ _ _ -> Ok (tx,None)
             costFn = fun _ _ _ _ -> 0L
             expiry=1000ul
             size=100ul
@@ -653,7 +653,7 @@ let ``contract get removed when expiring arrive``() =
     let contract : Contract.T =
         {
             hash=Contract.computeHash SampleContract.sampleContractCode
-            fn= fun _ _ _ _ tx -> Ok (tx,None)
+            mainFn= fun tx _ _ _ _ -> Ok (tx,None)
             costFn = fun _ _ _ _ -> 0L
             expiry=1ul
             size=100ul
